theories/tests/TestNat.v
@@ -444,19 +444,10 @@ with fuel : nat -> nat -> Prop :=
 | v1_step : forall (x v1 : nat), remFuel x v1 -> fuel (x) (v1).
 
 
-MetaRocq Run (animate_inductive v2 <?v2?> [("remFuel", ([0], [1])); ("fuel", ([0], [1])); ("v2", ([0], [1]))] 200).
-
-Example test_v2_0 :
-  v2AnimatedTopFn 50 (Success nat 0) = Success nat 0.
-Proof. reflexivity. Qed.
-
-Example test_v2_3 :
-  v2AnimatedTopFn 50 (Success nat 3) = Success nat 3.
-Proof. reflexivity. Qed.
-
-Example test_v2_5 :
-  v2AnimatedTopFn 50 (Success nat 5) = Success nat 5.
-Proof. reflexivity. Qed.
+(* Expected error: "relation name 'fuel' starts with an engine-reserved string"
+   The relation name 'fuel' is forbidden because the engine uses "fuel" as its
+   internal animation fuel-counter binder. *)
+Fail MetaRocq Run (animate_inductive v2 <?v2?> [("remFuel", ([0], [1])); ("fuel", ([0], [1])); ("v2", ([0], [1]))] 200).
 
 Inductive rel : nat -> nat -> Prop :=
 | x : forall v0 v1 , rel2 v0 v1 -> rel v0 v1
@@ -478,28 +469,20 @@ Proof. reflexivity. Qed.
 Example test_rel_5 :
   relAnimatedTopFn 50 (Success nat 5) = Success nat 5.
 Proof. reflexivity. Qed.
+End ClashRelName.
+Module clashFuel.
 
 Inductive v2' : nat -> nat -> Prop :=
-| vCon' : forall v0 v3 , fuel' v0 v3 -> v2' v0 v3
-with remFuel' : nat -> nat -> Prop :=
-| x_base'' : remFuel' 0 0
-| x_step'' : forall (v0 fuel : nat), remFuel' v0 fuel -> remFuel' (S v0) (S fuel)
-with fuel' : nat -> nat -> Prop :=
+| vCon' : forall v0 v3 , rel3 v0 v3 -> v2' v0 v3
+with v3 : nat -> nat -> Prop :=
+| x_base'' : v3 0 0
+| x_step'' : forall (v0 fuel : nat), v3 v0 fuel -> v3 (S v0) (S fuel)
+with rel3 : nat -> nat -> Prop :=
 
-| v1_step' : forall (x v1 : nat), remFuel' x v1 -> fuel' (x) (v1).
+| v1_step' : forall (x v1 : nat), v3 x v1 -> rel3 (x) (v1).
 
 
-MetaRocq Run (animate_inductive v2' <?v2'?> [("remFuel'", ([0], [1])); ("fuel'", ([0], [1])); ("v2'", ([0], [1]))] 200).
-
-Example test_v2'_0 :
-  v2'AnimatedTopFn 50 (Success nat 0) = Success nat 0.
-Proof. reflexivity. Qed.
-
-Example test_v2'_3 :
-  v2'AnimatedTopFn 50 (Success nat 3) = Success nat 3.
-Proof. reflexivity. Qed.
-
-Example test_v2'_5 :
-  v2'AnimatedTopFn 50 (Success nat 5) = Success nat 5.
-Proof. reflexivity. Qed.
-End ClashRelName.
+(* 
+    data-variable/relation-name disjointness check. *)
+Fail MetaRocq Run (animate_inductive v2' <?v2'?> [("v3", ([0], [1])); ("rel3", ([0], [1])); ("v2'", ([0], [1]))] 200).
+End clashFuel.
